@prefix bibo: <http://purl.org/ontology/bibo/> .
@prefix cc: <http://creativecommons.org/ns#> .
@prefix dcterms: <http://purl.org/dc/terms/> .
@prefix em: <http://emplaces.namespace.example.org/> .
@prefix eml: <http://emplaces.namespace.example.org/language/> .
@prefix emp: <http://emplaces.namespace.example.org/place/> .
@prefix emt: <http://emplaces.namespace.example.org/timespan/> .
@prefix foaf: <http://xmlns.com/foaf/0.1/> .
@prefix geonames: <http://sws.geonames.org/> .
@prefix gn: <http://www.geonames.org/ontology#> .
@prefix oa: <http://www.w3.org/ns/oa#> .
@prefix owl: <http://www.w3.org/2002/07/owl#> .
@prefix rdf: <http://www.w3.org/1999/02/22-rdf-syntax-ns#> .
@prefix rdfs: <http://www.w3.org/2000/01/rdf-schema#> .
@prefix skos: <http://www.w3.org/2004/02/skos/core#> .
@prefix wgs84_pos: <http://www.w3.org/2003/01/geo/wgs84_pos#> .
@prefix xml: <http://www.w3.org/XML/1998/namespace> .
@prefix xsd: <http://www.w3.org/2001/XMLSchema#> .

em:Place a rdfs:Class ;
    em:coreProperty em:alternateName,
        em:corePlaceType,
        em:placeCategory,
        em:preferredName .

em:AH_PART_OF_AH a em:Relation_type ;
    rdfs:label "Former part of" ;
    em:fromType em:P_OR_A ;
    em:toType gn:A ;
    rdfs:comment "Records a historical relationship between a historical place or administrative division and its parent division." .

em:APPROXIMATE a em:Competence_value ;
    rdfs:label "Approximate" ;
    rdfs:comment "The associated value is a date whose value is only approximately known.  @@NOTE: this value may prove spurious, as timespan already has a way to represent approximation ranges." .

em:ASSUMED a em:Competence_value ;
    rdfs:label "Assumed" ;
    rdfs:comment "The associated value is assumed from context." .

em:A_PART_OF_A a em:Relation_type ;
    rdfs:label "Subdivision of" ;
    em:fromType gn:A ;
    em:toType gn:A ;
    rdfs:comment "Relates a subdivision of an administrative division to its parent division." .

em:DEFINITIVE a em:Competence_value ;
    rdfs:label "Definitive" ;
    rdfs:comment "The associated value is definitively true for the purposes of EMPlaces.  Such information should ideally be backup up be appropiate source references." .

em:INFERRED a em:Competence_value ;
    rdfs:label "Inferred" ;
    rdfs:comment "The associated value has been inferred from (preferably?) definitive informaton." .

em:UNCERTAIN a em:Competence_value ;
    rdfs:label "Uncertain" ;
    rdfs:comment "The associated value is uncertain." .

em:competence a rdf:Property ;
    rdfs:label "Certainty, or quality, of information" ;
    rdfs:comment "Records the quality or certaintly of some information.  Note that in the absence of an explicit value, no competence should be assumed." ;
    rdfs:range em:Competence_value .

em:coreDataRef rdfs:subPropertyOf em:source .

eml:de a em:Language_value ;
    rdfs:label "German" ;
    em:tag "de" .

eml:la a em:Language_value ;
    rdfs:label "Latin" ;
    em:tag "la" .

eml:pl a em:Language_value ;
    rdfs:label "Polish" ;
    em:tag "pl" .

gn:A.ADM1H a skos:Concept ;
    rdfs:label "Former first-order admin division" ;
    rdfs:comment "A former first-order administrative division.  From GeoNames (feature code)." ;
    skos:narrower gn:A .

gn:A.ADM2H a skos:Concept ;
    rdfs:label "Former second-order admin division" ;
    rdfs:comment "A former first-order administrative division.  From GeoNames (feature code)." ;
    skos:narrower gn:A .

gn:A.ADM3H a skos:Concept ;
    rdfs:label "Former Third-order admin division" ;
    rdfs:comment "A former third-order administrative division.  From GeoNames (feature code)." ;
    skos:narrower gn:A .

gn:A.PCLH a skos:Concept ;
    rdfs:label "Former independent political entity" ;
    rdfs:comment "A former independent political entity, typically a country.  From GeoNames (feature code)." ;
    skos:narrower gn:A .

gn:P.PPL a skos:Concept ;
    rdfs:label "Populated place" ;
    rdfs:comment "A populated place (town, city, village, etc.).  From GeoNames (feature code)." ;
    skos:narrower gn:P .

gn:P.PPLH a skos:Concept ;
    rdfs:label "Former populated place" ;
    rdfs:comment "A former populated place that no longer exists.  From GeoNames (feature code)." ;
    skos:narrower gn:P .

em:P_OR_A a skos:Concept ;
    rdfs:label "Former populated place or admin division" ;
    rdfs:comment "Former populated place or administrative division, used in historical administrative relations" ;
    skos:broader gn:A,
        gn:P .

em:corePlaceType rdfs:subPropertyOf em:placeType .

gn:A.ADM1 a skos:Concept ;
    rdfs:label "First-order admin division" ;
    rdfs:comment "A primary administrative division of a country, such as a state in the United States.  From GeoNames (feature code)." ;
    skos:narrower gn:A .

gn:A.ADM2 a skos:Concept ;
    rdfs:label "Second-order admin division" ;
    rdfs:comment "A subdivision of a first-order administrative division.  From GeoNames (feature code)." ;
    skos:narrower gn:A .

gn:A.ADM3 a skos:Concept ;
    rdfs:label "Third-order admin division" ;
    rdfs:comment "A subdivision of a second-order administrative division.  From GeoNames (feature code)." ;
    skos:narrower gn:A .

gn:A.PCLI a skos:Concept ;
    rdfs:label "Independent political entity" ;
    rdfs:comment "An independent political entity, typically a country.  From GeoNames (feature code)." ;
    skos:narrower gn:A .

gn:P.PPLA a skos:Concept ;
    rdfs:label "Seat of 1st-order admin div" ;
    rdfs:comment "Populated place that is a seat of a first-order administrative division.  From GeoNames (feature code)." ;
    skos:narrower gn:P .

emp:g_3090048 a em:Place ;
    rdfs:label "Opole (seat of a first-order administrative division)" ;
    em:alternateName "Opole",
        "Oppein",
        "Oppeln",
        "أبولوسكي"@ar,
        "Горад Аполе"@be,
        "Ополе"@bg,
        "Opolí"@cs,
        "Òpòle"@csb,
        "Opole"@da,
        "Oppeln"@de,
        "Opole"@en,
        "Opole"@eo,
        "اوپوله"@fa,
        "Opole"@fi,
        "Opole"@fr,
        "אופולה"@he,
        "Opole"@hu,
        "Opole"@id,
        "Opole"@it,
        "オポーレ"@ja,
        "Opole"@jv,
        "오폴레"@ko,
        "Opolė"@lt,
        "Opole"@lv,
        "Opole"@na,
        "Oppeln"@nds,
        "Opole"@nl,
        "Opole"@pl,
        "اوپول"@pnb,
        "Opole"@pt,
        "Opole"@ro,
        "Ополе"@ru,
        "Opole"@sl,
        "Ополе"@sr,
        "Opole"@sv,
        "Uopole"@szl,
        "ออปอเล"@th,
        "Ополе"@uk,
        "奥波莱"@zh ;
    em:alternateURI [ rdfs:label "GeoNames URI" ;
            em:link <http://sws.geonames.org/3090048/> ] ;
    em:canonicalURI emp:g_3090048 ;
    em:coreDataRef [ rdfs:label "GeoNames data" ;
            em:link <http://sws.geonames.org/3090048/about.rdf> ] ;
    em:corePlaceType gn:P.PPLA ;
    em:displayName "Opole",
        "Opolí",
        "Opolė",
        "Oppein",
        "Oppeln",
        "Uopole",
        "Òpòle",
        "Горад Аполе",
        "Ополе",
        "אופולה",
        "أبولوسكي",
        "اوپول",
        "اوپوله",
        "ออปอเล",
        "オポーレ",
        "奥波莱",
        "오폴레" ;
    em:hasAnnotation [ a oa:Annotation ;
            em:source [ a em:Source_ref ;
                    rdfs:label "GeoNames data" ;
                    em:link <http://sws.geonames.org/3090048/about.rdf> ] ;
            em:when emt:Current ;
            oa:hasBody [ rdfs:label "Current map for Opole" ;
                    em:link <http://www.geonames.org/3090048/opole.html> ] ;
            oa:hasTarget emp:g_3090048 ;
            oa:motivatedBy em:MAP_RESOURCE ] ;
    em:hasRelation [ a em:Qualified_relation ;
            em:relationTo emp:g_7532413 ;
            em:relationType em:P_PART_OF_A ;
            em:source [ a em:Source_ref ;
                    rdfs:label "GeoNames data" ;
                    em:link <http://sws.geonames.org/3090048/about.rdf> ] ;
            em:when emt:Current ] ;
    em:placeCategory gn:P ;
    em:preferredName "Opole" ;
    em:where [ a em:Setting ;
            em:location [ a em:Location_value ;
                    wgs84_pos:lat 5.067211e+01 ;
                    wgs84_pos:long 1.792533e+01 ] ;
            em:source [ a em:Source_ref ;
                    rdfs:label "GeoNames data" ;
                    em:link <http://sws.geonames.org/3090048/about.rdf> ] ;
            em:when emt:Current ] ;
    rdfs:isDefinedBy <http://sws.geonames.org/3090048/about.rdf> ;
    rdfs:seeAlso <http://dbpedia.org/resource/Opole>,
        <http://en.wikipedia.org/wiki/Opole>,
        <http://ru.wikipedia.org/wiki/%D0%9E%D0%BF%D0%BE%D0%BB%D0%B5> .

emp:g_3337495 a em:Place ;
    rdfs:label "Opole Voivodeship (first-order administrative division)" ;
    em:alternateName "Województwo Opolskie",
        "Voivodat d'Opole"@ca,
        "Opolské vojvodství"@cs,
        "Òpòlsczé wòjewództwò"@csb,
        "Woiwodschaft Oppeln"@de,
        "Opole Voivodeship"@en,
        "Opolio"@eo,
        "Opole"@es,
        "Opole vojevoodkond"@et,
        "Voïvodie d'Opole"@fr,
        "Provinsi Opole"@id,
        "Voivodato di Opole"@it,
        "オポーレ県"@ja,
        "Opolės vaivadija"@lt,
        "Opole"@nl,
        "Województwo opolskie"@pl,
        "Província de Opole"@pt,
        "Voivodia de Opole"@pt,
        "Voievodatul Opole"@ro,
        "Опольское воеводство"@ru,
        "Opolské vojvodstvo"@sk,
        "Opole vojvodskap"@sv,
        "Opplen"@sv ;
    em:alternateURI [ rdfs:label "GeoNames URI" ;
            em:link <http://sws.geonames.org/3337495/> ] ;
    em:canonicalURI emp:g_3337495 ;
    em:coreDataRef [ rdfs:label "GeoNames data" ;
            em:link <http://sws.geonames.org/3337495/about.rdf> ] ;
    em:corePlaceType gn:A.ADM1 ;
    em:displayName "Opole",
        "Opole Voivodeship",
        "Opole vojevoodkond",
        "Opole vojvodskap",
        "Opolio",
        "Opolské vojvodstvo",
        "Opolské vojvodství",
        "Opolės vaivadija",
        "Opplen",
        "Provinsi Opole",
        "Província de Opole",
        "Voievodatul Opole",
        "Voivodat d'Opole",
        "Voivodato di Opole",
        "Voivodia de Opole",
        "Voïvodie d'Opole",
        "Woiwodschaft Oppeln",
        "Województwo Opolskie",
        "Województwo opolskie",
        "Òpòlsczé wòjewództwò",
        "Опольское воеводство",
        "オポーレ県" ;
    em:hasAnnotation [ a oa:Annotation ;
            em:source [ a em:Source_ref ;
                    rdfs:label "GeoNames data" ;
                    em:link <http://sws.geonames.org/3337495/about.rdf> ] ;
            em:when emt:Current ;
            oa:hasBody [ rdfs:label "Current map for Opole Voivodeship" ;
                    em:link <http://www.geonames.org/3337495/wojewodztwo-opolskie.html> ] ;
            oa:hasTarget emp:g_3337495 ;
            oa:motivatedBy em:MAP_RESOURCE ] ;
    em:hasRelation [ a em:Qualified_relation ;
            em:relationTo emp:g_3066138 ;
            em:relationType em:P_PART_OF_A ;
            em:source [ a em:Source_ref ;
                    rdfs:label "GeoNames data" ;
                    em:link <http://sws.geonames.org/3337495/about.rdf> ] ;
            em:when emt:Current ] ;
    em:placeCategory gn:A ;
    em:preferredName "Opole Voivodeship" ;
    em:where [ a em:Setting ;
            em:location [ a em:Location_value ;
                    wgs84_pos:lat 5.066667e+01 ;
                    wgs84_pos:long 1.79e+01 ] ;
            em:source [ a em:Source_ref ;
                    rdfs:label "GeoNames data" ;
                    em:link <http://sws.geonames.org/3337495/about.rdf> ] ;
            em:when emt:Current ] ;
    rdfs:isDefinedBy <http://sws.geonames.org/3337495/about.rdf> ;
    rdfs:seeAlso <http://dbpedia.org/resource/Opole_Voivodeship>,
        <http://en.wikipedia.org/wiki/Opole_Voivodeship>,
        <http://ru.wikipedia.org/wiki/%D0%9E%D0%BF%D0%BE%D0%BB%D1%8C%D1%81%D0%BA%D0%BE%D0%B5_%D0%B2%D0%BE%D0%B5%D0%B2%D0%BE%D0%B4%D1%81%D1%82%D0%B2%D0%BE> .

emp:g_798544 a em:Place ;
    rdfs:label "Poland (independent political entity)" ;
    em:alternateName "Lengyelország",
        "Lenkija",
        "Poland",
        "Polen",
        "Polija",
        "Polish People’s Republic",
        "Pologne",
        "Polonia",
        "Polsha",
        "Polska",
        "Polska Rzeczpospolita Ludowa",
        "Polsko",
        "Poola",
        "Pole"@af,
        "ፖላንድ"@am,
        "Polonia"@an,
        "Polaland"@ang,
        "بولندا"@ar,
        "ܦܘܠܢܕ"@arc,
        "Polonia"@ast,
        "Polşa"@az,
        "Польша"@be,
        "Полша"@bg,
        "পোল্যাণ্ড"@bn,
        "Polonia"@br,
        "Poljska"@bs,
        "Polònia"@ca,
        "Polsko"@cs,
        "Pòlskô"@csb,
        "Пол҄ьска"@cu,
        "Польша"@cv,
        "Gwlad Pwyl"@cy,
        "Polen"@da,
        "Polen"@de,
        "Polonya"@diq,
        "Πολωνία"@el,
        "Republic of Poland"@en,
        "Polio"@eo,
        "Pollando"@eo,
        "Polujo"@eo,
        "Poola"@et,
        "Polonia"@eu,
        "لهستان"@fa,
        "Puola"@fi,
        "Pólland"@fo,
        "Pologne"@frp,
        "Polonie"@fur,
        "Poalen"@fy,
        "An Pholainn"@ga,
        "A Phòlainn"@gd,
        "Polonia - Polska"@gl,
        "Polóña"@gn,
        "Yn Pholynn"@gv,
        "Poljska"@hbs,
        "פולין"@he,
        "पोलैंड"@hi,
        "Poljska"@hr,
        "Pólska"@hsb,
        "Lengyelország"@hu,
        "Լեհաստան"@hy,
        "Polonia"@ia,
        "Polandia"@id,
        "Polandia"@ilo,
        "Polonia"@io,
        "Pólland"@is,
        "Polonia"@it,
        "ポーランド"@ja,
        "polskas"@jbo,
        "Polandia"@jv,
        "პოლონეთი"@ka,
        "ប៉ូលូញ"@km,
        "폴란드"@ko,
        "Polonya"@ku,
        "Poloni"@kw,
        "Polonia"@la,
        "Polen"@lb,
        "Pole"@li,
        "Polonia"@lij,
        "ໂປແລນ"@lo,
        "Lenkija"@lt,
        "Polija"@lv,
        "Полска"@mk,
        "Poland"@ms,
        "Polonja"@mt,
        "Poran"@na,
        "Pulonnia"@nap,
        "Polen"@nb,
        "Polen"@nds,
        "Polen"@nl,
        "Polen"@nn,
        "Polen"@no,
        "Polonia"@nov,
        "Polongne"@nrm,
        "Polonha"@oc,
        "Pol’šu"@olo,
        "Польшæ"@os,
        "Polonya"@pam,
        "Rzeczpospolita Polska"@pl,
        "Polònia"@pms,
        "پولنډ"@ps,
        "Polónia"@pt,
        "Polônia"@pt,
        "Pulska"@qu,
        "Pulunya"@qu,
        "Polonia"@ro,
        "Полония"@ro,
        "Польша"@ru,
        "Polonia"@sc,
        "Pulonia"@scn,
        "Poland"@sco,
        "Polen"@se,
        "Poľsko"@sk,
        "Poljska"@sl,
        "Booland"@so,
        "Poloni"@sq,
        "Polonia"@sq,
        "Пољска"@sr,
        "Polen"@sv,
        "Poland"@sw,
        "போலந்து"@ta,
        "Polónia"@tet,
        "Лаҳистон"@tg,
        "ประเทศโปแลนด์"@th,
        "โปแลนด์"@th,
        "Polonya"@tl,
        "poland"@tl,
        "Polonya"@tr,
        "لەھىستان"@ug,
        "Польща"@uk,
        "Polsha"@uz,
        "Ba Lan"@vi,
        "Pooln"@vls,
        "Polän"@vo,
        "Polonya"@war,
        "פוילן"@yi,
        "波兰"@zh ;
    em:alternateURI [ rdfs:label "GeoNames URI" ;
            em:link <http://sws.geonames.org/798544/> ] ;
    em:canonicalURI emp:g_798544 ;
    em:coreDataRef [ rdfs:label "GeoNames data" ;
            em:link <http://sws.geonames.org/798544/about.rdf> ] ;
    em:corePlaceType gn:A.PCLI ;
    em:displayName "A Phòlainn",
        "An Pholainn",
        "Ba Lan",
        "Booland",
        "Gwlad Pwyl",
        "Lengyelország",
        "Lenkija",
        "Poalen",
        "Polaland",
        "Poland",
        "Polandia",
        "Pole",
        "Polen",
        "Polija",
        "Polio",
        "Polish People’s Republic",
        "Poljska",
        "Pollando",
        "Pologne",
        "Polongne",
        "Polonha",
        "Poloni",
        "Polonia",
        "Polonia - Polska",
        "Polonie",
        "Polonja",
        "Polonya",
        "Polsha",
        "Polska",
        "Polska Rzeczpospolita Ludowa",
        "Polsko",
        "Polujo",
        "Polän",
        "Polònia",
        "Polónia",
        "Polóña",
        "Polônia",
        "Polşa",
        "Pol’šu",
        "Poola",
        "Pooln",
        "Poran",
        "Poľsko",
        "Pulonia",
        "Pulonnia",
        "Pulska",
        "Pulunya",
        "Puola",
        "Pòlskô",
        "Pólland",
        "Pólska",
        "Republic of Poland",
        "Rzeczpospolita Polska",
        "Yn Pholynn",
        "poland",
        "polskas",
        "Πολωνία",
        "Лаҳистон",
        "Полония",
        "Полска",
        "Полша",
        "Польшæ",
        "Польша",
        "Польща",
        "Пол҄ьска",
        "Пољска",
        "Լեհաստան",
        "פוילן",
        "פולין",
        "بولندا",
        "لهستان",
        "لەھىستان",
        "پولنډ",
        "ܦܘܠܢܕ",
        "पोलैंड",
        "পোল্যাণ্ড",
        "போலந்து",
        "ประเทศโปแลนด์",
        "โปแลนด์",
        "ໂປແລນ",
        "პოლონეთი",
        "ፖላንድ",
        "ប៉ូលូញ",
        "ポーランド",
        "波兰",
        "폴란드" ;
    em:hasAnnotation [ a oa:Annotation ;
            em:source [ a em:Source_ref ;
                    rdfs:label "GeoNames data" ;
                    em:link <http://sws.geonames.org/798544/about.rdf> ] ;
            em:when emt:Current ;
            oa:hasBody [ rdfs:label "Current map for Poland" ;
                    em:link <http://www.geonames.org/798544/republic-of-poland.html> ] ;
            oa:hasTarget emp:g_798544 ;
            oa:motivatedBy em:MAP_RESOURCE ] ;
    em:hasRelation [ a em:Qualified_relation ;
            em:relationTo emp:g_7729884 ;
            em:relationType em:P_PART_OF_A ;
            em:source [ a em:Source_ref ;
                    rdfs:label "GeoNames data" ;
                    em:link <http://sws.geonames.org/798544/about.rdf> ] ;
            em:when emt:Current ] ;
    em:placeCategory gn:A ;
    em:preferredName "Poland" ;
    em:where [ a em:Setting ;
            em:location [ a em:Location_value ;
                    wgs84_pos:lat 5.2e+01 ;
                    wgs84_pos:long 2e+01 ] ;
            em:source [ a em:Source_ref ;
                    rdfs:label "GeoNames data" ;
                    em:link <http://sws.geonames.org/798544/about.rdf> ] ;
            em:when emt:Current ] ;
    rdfs:isDefinedBy <http://sws.geonames.org/798544/about.rdf> ;
    rdfs:seeAlso <http://dbpedia.org/resource/Poland>,
        <http://en.wikipedia.org/wiki/Poland>,
        <http://ru.wikipedia.org/wiki/%D0%9F%D0%BE%D0%BB%D0%BE%D0%BD%D0%B8%D1%8F>,
        <http://ru.wikipedia.org/wiki/%D0%9F%D0%BE%D0%BB%D1%8C%D1%88%D0%B0> .

emp:g_7530818 a em:Place ;
    rdfs:label "Opole (second-order administrative division)" ;
    em:alternateURI [ rdfs:label "GeoNames URI" ;
            em:link <http://sws.geonames.org/7530818/> ] ;
    em:canonicalURI emp:g_7530818 ;
    em:coreDataRef [ rdfs:label "GeoNames data" ;
            em:link <http://sws.geonames.org/7530818/about.rdf> ] ;
    em:corePlaceType gn:A.ADM2 ;
    em:hasAnnotation [ a oa:Annotation ;
            em:source [ a em:Source_ref ;
                    rdfs:label "GeoNames data" ;
                    em:link <http://sws.geonames.org/7530818/about.rdf> ] ;
            em:when emt:Current ;
            oa:hasBody [ rdfs:label "Current map for Opole" ;
                    em:link <http://www.geonames.org/7530818/opole.html> ] ;
            oa:hasTarget emp:g_7530818 ;
            oa:motivatedBy em:MAP_RESOURCE ] ;
    em:hasRelation [ a em:Qualified_relation ;
            em:relationTo emp:g_3082777 ;
            em:relationType em:P_PART_OF_A ;
            em:source [ a em:Source_ref ;
                    rdfs:label "GeoNames data" ;
                    em:link <http://sws.geonames.org/7530818/about.rdf> ] ;
            em:when emt:Current ] ;
    em:placeCategory gn:A ;
    em:preferredName "Opole" ;
    em:where [ a em:Setting ;
            em:location [ a em:Location_value ;
                    wgs84_pos:lat 5.065622e+01 ;
                    wgs84_pos:long 1.793066e+01 ] ;
            em:source [ a em:Source_ref ;
                    rdfs:label "GeoNames data" ;
                    em:link <http://sws.geonames.org/7530818/about.rdf> ] ;
            em:when emt:Current ] ;
    rdfs:isDefinedBy <http://sws.geonames.org/7530818/about.rdf> ;
    rdfs:seeAlso <http://dbpedia.org/resource/Opole>,
        <http://en.wikipedia.org/wiki/Opole> .

emp:g_7532413 a em:Place ;
    rdfs:label "Opole (third-order administrative division)" ;
    em:alternateURI [ rdfs:label "GeoNames URI" ;
            em:link <http://sws.geonames.org/7532413/> ] ;
    em:canonicalURI emp:g_7532413 ;
    em:coreDataRef [ rdfs:label "GeoNames data" ;
            em:link <http://sws.geonames.org/7532413/about.rdf> ] ;
    em:corePlaceType gn:A.ADM3 ;
    em:hasAnnotation [ a oa:Annotation ;
            em:source [ a em:Source_ref ;
                    rdfs:label "GeoNames data" ;
                    em:link <http://sws.geonames.org/7532413/about.rdf> ] ;
            em:when emt:Current ;
            oa:hasBody [ rdfs:label "Current map for Opole" ;
                    em:link <http://www.geonames.org/7532413/opole.html> ] ;
            oa:hasTarget emp:g_7532413 ;
            oa:motivatedBy em:MAP_RESOURCE ] ;
    em:hasRelation [ a em:Qualified_relation ;
            em:relationTo emp:g_7530818 ;
            em:relationType em:P_PART_OF_A ;
            em:source [ a em:Source_ref ;
                    rdfs:label "GeoNames data" ;
                    em:link <http://sws.geonames.org/7532413/about.rdf> ] ;
            em:when emt:Current ] ;
    em:placeCategory gn:A ;
    em:preferredName "Opole" ;
    em:where [ a em:Setting ;
            em:location [ a em:Location_value ;
                    wgs84_pos:lat 5.06562e+01 ;
                    wgs84_pos:long 1.79306e+01 ] ;
            em:source [ a em:Source_ref ;
                    rdfs:label "GeoNames data" ;
                    em:link <http://sws.geonames.org/7532413/about.rdf> ] ;
            em:when emt:Current ] ;
    rdfs:isDefinedBy <http://sws.geonames.org/7532413/about.rdf> ;
    rdfs:seeAlso <http://dbpedia.org/resource/Opole>,
        <http://en.wikipedia.org/wiki/Opole> .

em:P_PART_OF_A a em:Relation_type ;
    rdfs:label "Administered by" ;
    em:fromType gn:P ;
    em:toType gn:A ;
    rdfs:comment "Relates a populated place to its administrative division." .

gn:P a skos:Concept ;
    rdfs:label "Populated place" ;
    rdfs:comment "Populated place - from GeoNames (feature class)." .

emt:Current a em:Time_period ;
    rdfs:label "Current, as of 2018" ;
    em:timespan [ a em:Time_span ;
            <http://emplaces.namespace.example.org/earliestEnd:> "2018" ;
            <http://emplaces.namespace.example.org/latestStart:> "2018" ] ;
    rdfs:comment "For ease of retrieval, use this specific resource to label any current information (e.g. core data extracted from GeoNames).  Additional Timespan values could be indicated if required to convey more specific information." .

gn:A a skos:Concept ;
    rdfs:label "Administrative division" ;
    rdfs:comment "Administrative division - from GeoNames (feature class)." .


